squashme

TabularTypeInterpreter/Lemmas/Type/Basic.lean
@@ -4,6 +4,7 @@ import TabularTypeInterpreter.Semantics.Type
 namespace TabularTypeInterpreter
 
 open «F⊗⊕ω»
+open Std
 
 mutual
 
@@ -206,15 +207,40 @@ theorem TypeVar_open_TypeVar_close_id
     (add simp [TypeVar_open, TypeVar_close, TypeLambda.TypeVar_open, TypeLambda.TypeVar_close],
       50% cases TypeVarLocallyClosed, safe cases TypeLambda.TypeVarLocallyClosed)
 
+theorem TypeVar_open_drop
+  : m < n → (TypeVar_open τ a m).TypeVarLocallyClosed n → TypeVarLocallyClosed τ n := by
+  induction τ using rec_uniform generalizing m n <;> aesop
+    (add simp [TypeVar_open, TypeLambda.TypeVar_open], safe cases TypeVarLocallyClosed,
+      safe cases TypeLambda.TypeVarLocallyClosed, safe constructors TypeVarLocallyClosed,
+      safe constructors TypeLambda.TypeVarLocallyClosed)
+
 end TypeVarLocallyClosed
 
-theorem TypeVar_open_Monotype_open_comm (τ : Monotype) : TypeVarLocallyClosed τ' m → m ≠ n →
+theorem TypeVar_open_Monotype_open_comm (τ : Monotype) {τ'} : TypeVarLocallyClosed τ' m → m ≠ n →
     (τ.TypeVar_open a m).Monotype_open τ' n = (τ.Monotype_open τ' n).TypeVar_open a m := by
   induction τ using rec_uniform generalizing m n <;> aesop
     (add simp [TypeVar_open, Monotype_open, TypeLambda.TypeVar_open, TypeLambda.Monotype_open],
       20% [TypeVarLocallyClosed.TypeVar_open_id, Eq.symm, TypeVarLocallyClosed.weakening])
   · case left => exact a_1 _ _ a_5 |>.left a_2 a_3
   · case right => exact a_1 _ _ a_5 |>.right a_2 a_3
+
+theorem not_mem_freeTypeVars_TypeVar_open_intro
+  : a ∉ freeTypeVars τ → a ≠ a' → a ∉ (τ.TypeVar_open a' n).freeTypeVars := by
+  induction τ using rec_uniform generalizing n
+  case row ih =>
+    intro anin ne
+    rw [TypeVar_open, freeTypeVars]
+    simp [Function.comp]
+    intro I ξ τ mem eq
+    cases eq
+    have := ih (ξ, τ) mem
+    rw [freeTypeVars, List.mapMem_eq_map] at anin
+    let ⟨xninτ, xninξ⟩ := List.not_mem_append'.mp <|
+      List.not_mem_flatten.mp anin (τ.freeTypeVars ++ ξ.freeTypeVars) <|
+      List.mem_map.mpr ⟨(ξ, τ), mem, rfl⟩
+    exact List.not_mem_append'.mpr ⟨this.right xninτ ne, this.left xninξ ne⟩
+  all_goals aesop
+    (add simp [TypeVar_open, TypeLambda.TypeVar_open, freeTypeVars, TypeLambda.freeTypeVars])
 
 end Monotype
 
@@ -240,11 +266,25 @@ theorem TypeVar_open_sizeOf' (γ : QualifiedType) : (γ.TypeVar_open a n).sizeOf
   | .mono τ => rw [TypeVar_open, sizeOf', sizeOf', τ.TypeVar_open_sizeOf']
   | .qual ψ γ => rw [TypeVar_open, sizeOf', sizeOf', ψ.TypeVar_open_sizeOf', γ.TypeVar_open_sizeOf']
 
-theorem TypeVarLocallyClosed.TypeVar_open_TypeVar_close_id
+namespace TypeVarLocallyClosed
+
+theorem weakening (γlc : TypeVarLocallyClosed γ m) : TypeVarLocallyClosed γ (m + n) := by
+  induction γlc <;> aesop (simp_config := { arith := true })
+    (add safe constructors TypeVarLocallyClosed, 20% Monotype.TypeVarLocallyClosed.weakening)
+
+theorem TypeVar_open_TypeVar_close_id
   : TypeVarLocallyClosed γ n → (γ.TypeVar_close a n).TypeVar_open a n = γ := by
   induction γ <;> aesop
     (add simp [TypeVar_open, TypeVar_close], 50% cases TypeVarLocallyClosed,
       20% Monotype.TypeVarLocallyClosed.TypeVar_open_TypeVar_close_id)
+
+theorem TypeVar_open_drop
+  : m < n → (TypeVar_open γ a m).TypeVarLocallyClosed n → TypeVarLocallyClosed γ n := by
+  induction γ generalizing m n <;> aesop
+    (add simp TypeVar_open, safe cases TypeVarLocallyClosed, safe constructors TypeVarLocallyClosed,
+      20% Monotype.TypeVarLocallyClosed.TypeVar_open_drop)
+
+end TypeVarLocallyClosed
 
 theorem TypeVar_open_comm (γ : QualifiedType)
   : m ≠ n → (γ.TypeVar_open a m).TypeVar_open a' n = (γ.TypeVar_open a' n).TypeVar_open a m := by
@@ -255,6 +295,22 @@ theorem TypeVar_open_Monotype_open_comm (γ : QualifiedType) {τ : Monotype}
     (γ.TypeVar_open a m).Monotype_open τ n = (γ.Monotype_open τ n).TypeVar_open a m := by
   induction γ <;> aesop
     (add simp [TypeVar_open, Monotype_open], 20% Monotype.TypeVar_open_Monotype_open_comm)
+
+theorem not_mem_freeTypeVars_TypeVar_open_intro (anin : a ∉ freeTypeVars γ) (anea' : a ≠ a')
+  : a ∉ (γ.TypeVar_open a' n).freeTypeVars := by
+  match γ with
+  | .mono .. =>
+    rw [TypeVar_open]
+    rw [freeTypeVars] at anin ⊢
+    exact Monotype.not_mem_freeTypeVars_TypeVar_open_intro anin anea'
+  | .qual .. =>
+    rw [TypeVar_open]
+    rw [freeTypeVars] at anin ⊢
+    let ⟨aninψ, aninγ'⟩ := List.not_mem_append'.mp anin
+    exact List.not_mem_append'.mpr ⟨
+      Monotype.not_mem_freeTypeVars_TypeVar_open_intro aninψ anea',
+      not_mem_freeTypeVars_TypeVar_open_intro aninγ' anea'
+    ⟩
 
 end QualifiedType
 
@@ -275,11 +331,29 @@ theorem TypeVar_open_sizeOf' (σ : TypeScheme) : (σ.TypeVar_open a n).sizeOf' =
   | .qual γ => rw [TypeVar_open, sizeOf', sizeOf', γ.TypeVar_open_sizeOf']
   | .quant _ σ => rw [TypeVar_open, sizeOf', sizeOf', σ.TypeVar_open_sizeOf']
 
-theorem TypeVarLocallyClosed.TypeVar_open_TypeVar_close_id
+namespace TypeVarLocallyClosed
+
+theorem weakening (σlc : TypeVarLocallyClosed σ m) : TypeVarLocallyClosed σ (m + n) := by
+  induction σlc <;> aesop (simp_config := { arith := true })
+    (add safe constructors TypeVarLocallyClosed,
+      20% [of_eq, QualifiedType.TypeVarLocallyClosed.weakening])
+where
+  of_eq {σ m n} (σlc : TypeVarLocallyClosed σ m) (eq : m = n) : σ.TypeVarLocallyClosed n := by
+    rwa [eq] at σlc
+
+theorem TypeVar_open_TypeVar_close_id
   : TypeVarLocallyClosed σ n → (σ.TypeVar_close a n).TypeVar_open a n = σ  := by
   induction σ generalizing n <;> aesop
     (add simp [TypeVar_open, TypeVar_close], 50% cases TypeVarLocallyClosed,
       20% [QualifiedType.TypeVarLocallyClosed.TypeVar_open_TypeVar_close_id])
+
+theorem TypeVar_open_drop
+  : m < n → (TypeVar_open σ a m).TypeVarLocallyClosed n → TypeVarLocallyClosed σ n := by
+  induction σ generalizing m n <;> aesop
+    (add simp TypeVar_open, safe cases TypeVarLocallyClosed, safe constructors TypeVarLocallyClosed,
+      20% QualifiedType.TypeVarLocallyClosed.TypeVar_open_drop)
+
+end TypeVarLocallyClosed
 
 theorem TypeVar_open_comm (σ : TypeScheme)
   : m ≠ n → (σ.TypeVar_open a m).TypeVar_open a' n = (σ.TypeVar_open a' n).TypeVar_open a m := by
@@ -292,6 +366,18 @@ theorem TypeVar_open_Monotype_open_comm (σ : TypeScheme) {τ : Monotype}
   induction σ generalizing m n <;> aesop
     (add simp [TypeVar_open, Monotype_open],
       20% [QualifiedType.TypeVar_open_Monotype_open_comm, Monotype.TypeVarLocallyClosed.weakening])
+
+theorem not_mem_freeTypeVars_TypeVar_open_intro (anin : a ∉ freeTypeVars σ) (anea' : a ≠ a')
+  : a ∉ (σ.TypeVar_open a' n).freeTypeVars := by
+  match σ with
+  | .qual _ =>
+    rw [TypeVar_open]
+    rw [freeTypeVars] at anin ⊢
+    exact QualifiedType.not_mem_freeTypeVars_TypeVar_open_intro anin anea'
+  | .quant .. =>
+    rw [TypeVar_open]
+    rw [freeTypeVars] at anin ⊢
+    exact not_mem_freeTypeVars_TypeVar_open_intro anin anea'
 
 namespace KindingAndElaboration
 
@@ -344,13 +430,71 @@ theorem row_inversion
     ⟩
   ⟩
 
+theorem TypeVarLocallyClosed_of (σke : [[Γc; Γ ⊢ σ : κ ⇝ A]]) : σ.TypeVarLocallyClosed := by
+  induction σke using
+    rec (motive_2 := fun _ _ _ _ => True) (motive_3 := fun _ _ => ∀ {x : True}, True)
+  case scheme I _ _ ih =>
+    let ⟨a, anin⟩ := I.exists_fresh
+    exact .quant <| ih a anin |>.weakening.TypeVar_open_drop Nat.zero_lt_one
+  case row => exact .qual <| .mono <| .row sorry -- TODO: Fix generation of this constructor.
+  case lift I _ _ _ ih₀ ih₁ =>
+    let ⟨a, anin⟩ := I.exists_fresh
+    let .qual (.mono τlc) := ih₀ a anin
+    let .qual (.mono ρlc) := ih₁
+    exact .qual <| .mono <| .lift (.mk <| τlc.weakening.TypeVar_open_drop Nat.one_pos) ρlc
+  case ind ih₀ _ _ =>
+    let .qual (.mono ρlc) := ih₀
+    exact .qual <| .mono <| .ind ρlc
+  case all I _ _ _ ih₀ ih₁ =>
+    let ⟨a, anin⟩ := I.exists_fresh
+    let .qual (.mono ψlc) := ih₀ a anin
+    let .qual (.mono ρlc) := ih₁
+    exact .qual <| .mono <| .all (.mk <| ψlc.weakening.TypeVar_open_drop Nat.one_pos) ρlc
+  case split ih =>
+    let .qual (.mono (.concat (.lift «λτlc» ρ₀lc) _ ρ₁lc ρ₂lc)) := ih
+    exact .qual <| .mono <| .split «λτlc» ρ₀lc ρ₁lc ρ₂lc
+  all_goals aesop (add safe cases TypeVarLocallyClosed,
+    40% cases QualifiedType.TypeVarLocallyClosed, safe constructors TypeVarLocallyClosed,
+    safe constructors QualifiedType.TypeVarLocallyClosed,
+    safe constructors Monotype.TypeVarLocallyClosed)
+
 end KindingAndElaboration
 
 end TypeScheme
 
-def Monotype.label.Uniqueness.Perm_preservation {ξ' : Nat → Monotype}
-  (uni : [[unique(</ ξ@i // i in [:n] />)]]) (perm : List.Perm p [:n])
-  (eq : ∀ i, ξ' i = ξ (p.get! i)) : [[unique(</ ξ'@i // i in [:n] />)]] := by
+namespace Monotype.label.Uniqueness
+
+local instance : Inhabited Monotype where
+  default := .row [] none
+in
+def Monotype_open_preservation (uni : Uniqueness (List.map (TypeVar_open · a n) ξ))
+  : Uniqueness (ξ.map (·.Monotype_open τ n)) := by
+  generalize ξ'eq : ξ.map (·.TypeVar_open a n) = ξ' at uni
+  match uni with
+  | concrete ne (ℓ := ℓ) =>
+    rw [List.map_singleton_flatten] at ξ'eq
+    let length_eq : List.length (List.map ..) = List.length _ := by rw [ξ'eq]
+    rw [List.length_map, List.length_map, Range.length_toList, Nat.sub_zero] at length_eq
+    rw [← Range.map_get!_eq (as := ξ), length_eq, List.map_map] at ξ'eq ⊢
+    rw [Range.map_eq_of_eq_of_mem (by
+      intro i mem
+      simp only [Function.comp]
+      show _ = .label (ℓ i)
+      have := Range.eq_of_mem_of_map_eq ξ'eq i mem
+      simp only [Function.comp] at this
+      generalize ξ''eq : ξ.get! i = ξ'' at *
+      cases ξ'' <;> rw [TypeVar_open] at this
+      case label => rw [Monotype_open, label.inj this]
+      all_goals nomatch this
+    ), ← List.map_singleton_flatten, ← Range.map]
+    exact concrete ne
+  | var =>
+    let [_] := ξ
+    exact var
+
+def Perm_preservation {ξ' : Nat → Monotype} (uni : [[unique(</ ξ@i // i in [:n] />)]])
+  (perm : List.Perm p [:n]) (eq : ∀ i, ξ' i = ξ (p.get! i))
+  : [[unique(</ ξ'@i // i in [:n] />)]] := by
   generalize ξseq : ([:n].map fun i => [ξ i]).flatten = ξs at uni
   match uni with
   | concrete ne (ℓ := ℓ) =>
@@ -396,5 +540,7 @@ def Monotype.label.Uniqueness.Perm_preservation {ξ' : Nat → Monotype}
         Std.Range.toList, if_neg (nomatch ·), Nat.zero_add,
         if_neg (Nat.not_lt_of_le (Nat.le_refl _)), List.map_singleton]
     exact var
+
+end Monotype.label.Uniqueness
 
 end TabularTypeInterpreter
