TabularTypeInterpreter/Lemmas/Type/MonotypeOpenPreservation.lean
@@ -3,15 +3,1027 @@ import TabularTypeInterpreter.Lemmas.TypeEnvironment
 import TabularTypeInterpreter.Theorems.Kind
 import TabularTypeInterpreter.Theorems.Type.KindingAndElaboration
 
-namespace TabularTypeInterpreter.TypeScheme.KindingAndElaboration
+namespace TabularTypeInterpreter
+
+open Std
+
+namespace «F⊗⊕ω».Type
+
+private
+theorem contain_evidence_eq_inversion (aninA : a ∉ A.freeTypeVars)
+  (eq : A.TypeVar_open a n = [[⊗ {∀ a : K ↦ *. (⊗ (a$0 ⟦A₁⟧)) → ⊗ (a$0 ⟦A₀⟧), ∀ a : K ↦ *. (⊕ (a$0 ⟦A₀⟧)) → ⊕ (a$0 ⟦A₁⟧)}]])
+  : ∃ A₀' A₁', A₀ = A₀'.TypeVar_open a (n + 1) ∧ A₁ = A₁'.TypeVar_open a (n + 1) ∧
+    A = [[⊗ {∀ a : K ↦ *. (⊗ (a$0 ⟦A₁'⟧)) → ⊗ (a$0 ⟦A₀'⟧), ∀ a : K ↦ *. (⊕ (a$0 ⟦A₀'⟧)) → ⊕ (a$0 ⟦A₁'⟧)}]] := by
+  cases A <;> rw [TypeVar_open] at *
+  case prod =>
+    rename «Type» => A
+    let eq' := prod.inj eq
+    cases A <;> rw [TypeVar_open] at *
+    case list =>
+      let eq'' := list.inj eq'
+      rw [List.mapMem_eq_map] at *
+      rename List _ => As
+      match As with
+      | [] => nomatch eq''
+      | A₀' :: As' =>
+        rw [List.map_cons] at *
+        match As' with
+        | [] =>
+          generalize A₀'.TypeVar_open a n = A₀'' at *
+          nomatch eq''
+        | A₁' :: As'' =>
+          rw [List.map_cons] at *
+          match As'' with
+          | A₂' :: _ =>
+            generalize A₀'.TypeVar_open a n = A₀'' at *
+            generalize A₁'.TypeVar_open a n = A₁'' at *
+            generalize A₂'.TypeVar_open a n = A₂'' at *
+            nomatch eq''
+          | [] =>
+            rw [List.map_nil] at *
+            let ⟨eq₀, eq'''⟩ := List.cons_eq_cons.mp eq''
+            let eq₁ := List.singleton_inj.mp eq'''
+            cases A₀' <;> rw [TypeVar_open] at *
+            case «forall» =>
+              let ⟨Keq, eq₀'⟩ := forall.inj eq₀
+              cases Keq
+              rename «Type» => A₀'
+              cases A₀' <;> rw [Type.TypeVar_open] at *
+              case arr =>
+                rename_i A₀₀' A₀₁'
+                cases A₀₀' <;> rw [Type.TypeVar_open] at *
+                case prod =>
+                  rename «Type» => A₀₀'
+                  cases A₀₀' <;> rw [Type.TypeVar_open] at *
+                  case listApp =>
+                    rename_i A₀₀₀' A₀₀₁'
+                    cases A₀₀₀' <;> rw [Type.TypeVar_open] at *
+                    case var =>
+                      rename «F⊗⊕ω».TypeVar => a'
+                      cases a'
+                      case bound =>
+                        rename Nat => n'
+                        match n' with
+                        | 0 =>
+                          rw [if_neg (nomatch ·)] at *
+                          cases A₀₁' <;> rw [Type.TypeVar_open] at *
+                          case prod =>
+                            rename «Type» => A₀₀'
+                            cases A₀₀' <;> rw [Type.TypeVar_open] at *
+                            case listApp =>
+                              rename_i A₀₁₀' A₀₁₁'
+                              cases A₀₁₀' <;> rw [Type.TypeVar_open] at *
+                              case var =>
+                                rename «F⊗⊕ω».TypeVar => a'
+                                cases a'
+                                case bound =>
+                                  rename Nat => n'
+                                  match n' with
+                                  | 0 =>
+                                    rw [if_neg (nomatch ·)] at *
+                                    cases A₁' <;> rw [TypeVar_open] at *
+                                    case «forall» =>
+                                      let ⟨Keq, eq₁'⟩ := forall.inj eq₁
+                                      cases Keq
+                                      rename «Type» => A₁'
+                                      cases A₁' <;> rw [Type.TypeVar_open] at *
+                                      case arr =>
+                                        rename_i A₁₀' A₁₁'
+                                        cases A₁₀' <;> rw [Type.TypeVar_open] at *
+                                        case sum =>
+                                          rename «Type» => A₁₀'
+                                          cases A₁₀' <;> rw [Type.TypeVar_open] at *
+                                          case listApp =>
+                                            rename_i A₁₀₀' A₁₀₁'
+                                            cases A₁₀₀' <;> rw [Type.TypeVar_open] at *
+                                            case var =>
+                                              rename «F⊗⊕ω».TypeVar => a'
+                                              cases a'
+                                              case bound =>
+                                                rename Nat => n'
+                                                match n' with
+                                                | 0 =>
+                                                  rw [if_neg (nomatch ·)] at *
+                                                  cases A₁₁' <;> rw [Type.TypeVar_open] at *
+                                                  case sum =>
+                                                    rename «Type» => A₁₀'
+                                                    cases A₁₀' <;> rw [Type.TypeVar_open] at *
+                                                    case listApp =>
+                                                      rename_i A₁₁₀' A₁₁₁'
+                                                      cases A₁₁₀' <;> rw [Type.TypeVar_open] at *
+                                                      case var =>
+                                                        rename «F⊗⊕ω».TypeVar => a'
+                                                        cases a'
+                                                        case bound =>
+                                                          rename Nat => n'
+                                                          match n' with
+                                                          | 0 =>
+                                                            rw [if_neg (nomatch ·)] at *
+                                                            cases eq₀'
+                                                            let ⟨eq₁₀, eq₁₁⟩ := arr.inj eq₁'
+                                                            simp [freeTypeVars] at aninA
+                                                            let ⟨
+                                                              aninA₀₀₁',
+                                                              aninA₀₁₁',
+                                                              aninA₁₀₁',
+                                                              aninA₁₁₁'
+                                                            ⟩ := aninA
+                                                            cases
+                                                              TypeVar_open_inj_of_not_mem_freeTypeVars
+                                                              aninA₁₀₁' aninA₀₁₁' <| And.right <|
+                                                              listApp.inj <| sum.inj eq₁₀
+                                                            cases
+                                                              TypeVar_open_inj_of_not_mem_freeTypeVars
+                                                              aninA₁₁₁' aninA₀₀₁' <| And.right <|
+                                                              listApp.inj <| sum.inj eq₁₁
+                                                            exact ⟨_, _, rfl, rfl, rfl⟩
+                                                          | _ + 1 => split at eq₁' <;> nomatch eq₁'
+                                                        all_goals nomatch eq₁'
+                                                      all_goals nomatch eq₁'
+                                                    all_goals nomatch eq₁'
+                                                  all_goals nomatch eq₁'
+                                                | _ + 1 => split at eq₁' <;> nomatch eq₁'
+                                              all_goals nomatch eq₁'
+                                            all_goals nomatch eq₁'
+                                          all_goals nomatch eq₁'
+                                        all_goals nomatch eq₁'
+                                      all_goals nomatch eq₁'
+                                    all_goals nomatch eq₁
+                                  | _ + 1 => split at eq₀' <;> nomatch eq₀'
+                                all_goals nomatch eq₀'
+                              all_goals nomatch eq₀'
+                            all_goals nomatch eq₀'
+                          all_goals nomatch eq₀'
+                        | _ + 1 => split at eq₀' <;> nomatch eq₀'
+                      all_goals nomatch eq₀'
+                    all_goals nomatch eq₀'
+                  all_goals nomatch eq₀'
+                all_goals nomatch eq₀'
+              all_goals nomatch eq₀'
+            all_goals nomatch eq₀
+    all_goals nomatch eq
+  all_goals nomatch eq
+
+private
+theorem concat_evidence_eq_inversion (aninA : a ∉ A.freeTypeVars)
+  (eq : A.TypeVar_open a n = [[⊗ {∀ a : K ↦ *. (⊗ (a$0 ⟦A₀⟧)) → (⊗ (a$0 ⟦A₁⟧)) → ⊗ (a$0 ⟦A₂⟧), ∀ a : K ↦ *. ∀ aₜ : *. ((⊕ (a$1 ⟦A₀⟧)) → aₜ$0) → ((⊕ (a$1 ⟦A₁⟧)) → aₜ$0) → (⊕ (a$1 ⟦A₂⟧)) → aₜ$0, Bₗ, Bᵣ}]])
+  : ∃ A₀' A₁' A₂' Bₗ' Bᵣ', A₀ = A₀'.TypeVar_open a (n + 1) ∧ A₁ = A₁'.TypeVar_open a (n + 1) ∧
+    A₂ = A₂'.TypeVar_open a (n + 1) ∧
+    Bₗ = Bₗ'.TypeVar_open a n ∧ Bᵣ = Bᵣ'.TypeVar_open a n ∧
+    A = [[⊗ {∀ a : K ↦ *. (⊗ (a$0 ⟦A₀'⟧)) → (⊗ (a$0 ⟦A₁'⟧)) → ⊗ (a$0 ⟦A₂'⟧), ∀ a : K ↦ *. ∀ aₜ : *. ((⊕ (a$1 ⟦A₀'⟧)) → aₜ$0) → ((⊕ (a$1 ⟦A₁'⟧)) → aₜ$0) → (⊕ (a$1 ⟦A₂'⟧)) → aₜ$0, Bₗ', Bᵣ'}]] := by
+  cases A <;> rw [TypeVar_open] at *
+  case prod =>
+    rename «Type» => A
+    let eq' := prod.inj eq
+    cases A <;> rw [TypeVar_open] at *
+    case list =>
+      let eq'' := list.inj eq'
+      rw [List.mapMem_eq_map] at *
+      rename List _ => As
+      match As with
+      | [] => nomatch eq''
+      | A₀' :: As' =>
+        rw [List.map_cons] at *
+        match As' with
+        | [] =>
+          generalize A₀'.TypeVar_open a n = A₀'' at *
+          nomatch eq''
+        | A₁' :: As'' =>
+          rw [List.map_cons] at *
+          match As'' with
+          | [] =>
+            generalize A₀'.TypeVar_open a n = A₀'' at *
+            generalize A₁'.TypeVar_open a n = A₁'' at *
+            nomatch eq''
+          | Bₗ' :: As'' =>
+            rw [List.map_cons] at *
+            match As'' with
+            | [] =>
+              generalize A₀'.TypeVar_open a n = A₀'' at *
+              generalize A₁'.TypeVar_open a n = A₁'' at *
+              generalize Bₗ'.TypeVar_open a n = Bₗ'' at *
+              nomatch eq''
+            | Bᵣ' :: As'' =>
+              rw [List.map_cons] at *
+              match As'' with
+              | A₅' :: As'' =>
+                generalize A₀'.TypeVar_open a n = A₀'' at *
+                generalize A₁'.TypeVar_open a n = A₁'' at *
+                generalize Bₗ'.TypeVar_open a n = Bₗ'' at *
+                generalize Bᵣ'.TypeVar_open a n = Bᵣ'' at *
+                generalize A₅'.TypeVar_open a n = A₅'' at *
+                nomatch eq''
+              | [] =>
+                rw [List.map_nil] at *
+                let ⟨eq₀, eq'''⟩ := List.cons_eq_cons.mp eq''
+                let ⟨eq₁, eq''''⟩ := List.cons_eq_cons.mp eq'''
+                cases A₀' <;> rw [TypeVar_open] at *
+                case «forall» =>
+                  let ⟨Keq, eq₀'⟩ := forall.inj eq₀
+                  cases Keq
+                  rename «Type» => A₀'
+                  cases A₀' <;> rw [TypeVar_open] at *
+                  case arr =>
+                    rename_i A₀₀' A₀₁'
+                    cases A₀₀' <;> rw [Type.TypeVar_open] at *
+                    case prod =>
+                      rename «Type» => A₀₀'
+                      cases A₀₀' <;> rw [Type.TypeVar_open] at *
+                      case listApp =>
+                        rename_i A₀₀₀' A₀₀₁'
+                        cases A₀₀₀' <;> rw [Type.TypeVar_open] at *
+                        case var =>
+                          rename «F⊗⊕ω».TypeVar => a'
+                          cases a'
+                          case bound =>
+                            rename Nat => n'
+                            match n' with
+                            | 0 =>
+                              rw [if_neg (nomatch ·)] at *
+                              cases A₀₁' <;> rw [Type.TypeVar_open] at *
+                              case arr =>
+                                rename_i A₀₁₀' A₀₁₁'
+                                cases A₀₁₀' <;> rw [Type.TypeVar_open] at *
+                                case prod =>
+                                  rename «Type» => A₀₁₀'
+                                  cases A₀₁₀' <;> rw [Type.TypeVar_open] at *
+                                  case listApp =>
+                                    rename_i A₀₁₀₀' A₀₁₀₁'
+                                    cases A₀₁₀₀' <;> rw [Type.TypeVar_open] at *
+                                    case var =>
+                                      rename «F⊗⊕ω».TypeVar => a'
+                                      cases a'
+                                      case bound =>
+                                        rename Nat => n'
+                                        match n' with
+                                        | 0 =>
+                                          rw [if_neg (nomatch ·)] at *
+                                          cases A₀₁₁' <;> rw [Type.TypeVar_open] at *
+                                          case prod =>
+                                            rename «Type» => A₀₁₁'
+                                            cases A₀₁₁' <;> rw [Type.TypeVar_open] at *
+                                            case listApp =>
+                                              rename_i A₀₁₁₀' A₀₁₁₁'
+                                              cases A₀₁₁₀' <;> rw [Type.TypeVar_open] at *
+                                              case var =>
+                                                rename «F⊗⊕ω».TypeVar => a'
+                                                cases a'
+                                                case bound =>
+                                                  rename Nat => n'
+                                                  match n' with
+                                                  | 0 =>
+                                                    rw [if_neg (nomatch ·)] at *
+                                                    cases A₁' <;> rw [TypeVar_open] at *
+                                                    case «forall» =>
+                                                      let ⟨Keq, eq₁'⟩ := forall.inj eq₁
+                                                      cases Keq
+                                                      rename «Type» => A₁'
+                                                      cases A₁' <;> rw [TypeVar_open] at *
+                                                      case «forall» =>
+                                                        let ⟨Keq, eq₁''⟩ := forall.inj eq₁'
+                                                        cases Keq
+                                                        rename «Type» => A₁'
+                                                        cases A₁' <;> rw [TypeVar_open] at *
+                                                        case arr =>
+                                                          rename_i A₁₀' A₁₁'
+                                                          cases A₁₀' <;> rw [TypeVar_open] at *
+                                                          case arr =>
+                                                            rename_i A₁₀₀' A₁₀₁'
+                                                            cases A₁₀₀' <;> rw [TypeVar_open] at *
+                                                            case sum =>
+                                                              rename «Type» => A₁₀₀'
+                                                              cases A₁₀₀' <;> rw [TypeVar_open] at *
+                                                              case listApp =>
+                                                                rename_i A₁₀₀₀' A₁₀₀₁'
+                                                                cases A₁₀₀₀' <;> rw [Type.TypeVar_open] at *
+                                                                case var =>
+                                                                  rename «F⊗⊕ω».TypeVar => a'
+                                                                  cases a'
+                                                                  case bound =>
+                                                                    rename Nat => n'
+                                                                    match n' with
+                                                                    | 1 =>
+                                                                      rw [if_neg (nomatch ·)] at *
+                                                                      cases A₁₀₁' <;> rw [Type.TypeVar_open] at *
+                                                                      case var =>
+                                                                        rename «F⊗⊕ω».TypeVar => a'
+                                                                        cases a'
+                                                                        case bound =>
+                                                                          rename Nat => n'
+                                                                          match n' with
+                                                                          | 0 =>
+                                                                            rw [if_neg (nomatch ·)] at *
+                                                                            cases A₁₁' <;> rw [Type.TypeVar_open] at *
+                                                                            case arr =>
+                                                                              rename_i A₁₁₀' A₁₁₁'
+                                                                              cases A₁₁₀' <;> rw [TypeVar_open] at *
+                                                                              case arr =>
+                                                                                rename_i A₁₁₀₀' A₁₁₀₁'
+                                                                                cases A₁₁₀₀' <;> rw [TypeVar_open] at *
+                                                                                case sum =>
+                                                                                  rename «Type» => A₁₁₀₀'
+                                                                                  cases A₁₁₀₀' <;> rw [TypeVar_open] at *
+                                                                                  case listApp =>
+                                                                                    rename_i A₁₁₀₀₀' A₁₁₀₀₁'
+                                                                                    cases A₁₁₀₀₀' <;> rw [Type.TypeVar_open] at *
+                                                                                    case var =>
+                                                                                      rename «F⊗⊕ω».TypeVar => a'
+                                                                                      cases a'
+                                                                                      case bound =>
+                                                                                        rename Nat => n'
+                                                                                        match n' with
+                                                                                        | 1 =>
+                                                                                          rw [if_neg (nomatch ·)] at *
+                                                                                          cases A₁₁₀₁' <;> rw [Type.TypeVar_open] at *
+                                                                                          case var =>
+                                                                                            rename «F⊗⊕ω».TypeVar => a'
+                                                                                            cases a'
+                                                                                            case bound =>
+                                                                                              rename Nat => n'
+                                                                                              match n' with
+                                                                                              | 0 =>
+                                                                                                rw [if_neg (nomatch ·)] at *
+                                                                                                cases A₁₁₁' <;> rw [TypeVar_open] at *
+                                                                                                case arr =>
+                                                                                                  rename_i A₁₁₁₀' A₁₁₁₁'
+                                                                                                  cases A₁₁₁₀' <;> rw [TypeVar_open] at *
+                                                                                                  case sum =>
+                                                                                                    rename «Type» => A₁₁₁₀'
+                                                                                                    cases A₁₁₁₀' <;> rw [TypeVar_open] at *
+                                                                                                    case listApp =>
+                                                                                                      rename_i A₁₁₁₀₀' A₁₁₁₀₁'
+                                                                                                      cases A₁₁₁₀₀' <;> rw [Type.TypeVar_open] at *
+                                                                                                      case var =>
+                                                                                                        rename «F⊗⊕ω».TypeVar => a'
+                                                                                                        cases a'
+                                                                                                        case bound =>
+                                                                                                          rename Nat => n'
+                                                                                                          match n' with
+                                                                                                          | 1 =>
+                                                                                                            rw [if_neg (nomatch ·)] at *
+                                                                                                            cases A₁₁₁₁' <;> rw [Type.TypeVar_open] at *
+                                                                                                            case var =>
+                                                                                                              rename «F⊗⊕ω».TypeVar => a'
+                                                                                                              cases a'
+                                                                                                              case bound =>
+                                                                                                                rename Nat => n'
+                                                                                                                match n' with
+                                                                                                                | 0 =>
+                                                                                                                  rw [if_neg (nomatch ·)] at *
+                                                                                                                  cases eq₀'
+                                                                                                                  let ⟨eq₁₀, eq₁₁⟩ := arr.inj eq₁''
+                                                                                                                  let ⟨eq₁₁₀, eq₁₁₁⟩ := arr.inj eq₁₁
+                                                                                                                  simp [freeTypeVars] at aninA
+                                                                                                                  let ⟨
+                                                                                                                    aninA₀₀₁',
+                                                                                                                    aninA₀₁₀₁',
+                                                                                                                    aninA₀₁₁₁',
+                                                                                                                    aninA₁₀₀₁',
+                                                                                                                    aninA₁₁₀₀₁',
+                                                                                                                    aninA₁₁₁₀₁',
+                                                                                                                    aninBₗ,
+                                                                                                                    aninBᵣ
+                                                                                                                  ⟩ := aninA
+                                                                                                                  let f := And.right <| listApp.inj <| sum.inj <| And.left <| arr.inj eq₁₀
+                                                                                                                  sorry
+                                                                                                                | _ + 1 => split at eq₁'' <;> nomatch eq₁''
+                                                                                                              all_goals nomatch eq₁''
+                                                                                                            all_goals nomatch eq₁''
+                                                                                                          | 0 | _ + 2 => split at eq₁'' <;> nomatch eq₁''
+                                                                                                        all_goals nomatch eq₁''
+                                                                                                      all_goals nomatch eq₁''
+                                                                                                    all_goals nomatch eq₁''
+                                                                                                  all_goals nomatch eq₁''
+                                                                                                all_goals nomatch eq₁''
+                                                                                              | _ + 1 => split at eq₁'' <;> nomatch eq₁''
+                                                                                            all_goals nomatch eq₁''
+                                                                                          all_goals nomatch eq₁''
+                                                                                        | 0 | _ + 2 => split at eq₁'' <;> nomatch eq₁''
+                                                                                      all_goals nomatch eq₁''
+                                                                                    all_goals nomatch eq₁''
+                                                                                  all_goals nomatch eq₁''
+                                                                                all_goals nomatch eq₁''
+                                                                              all_goals nomatch eq₁''
+                                                                            all_goals nomatch eq₁''
+                                                                          | _ + 1 => split at eq₁'' <;> nomatch eq₁''
+                                                                        all_goals nomatch eq₁''
+                                                                      all_goals nomatch eq₁''
+                                                                    | 0 | _ + 2 => split at eq₁'' <;> nomatch eq₁''
+                                                                  all_goals nomatch eq₁''
+                                                                all_goals nomatch eq₁''
+                                                              all_goals nomatch eq₁''
+                                                            all_goals nomatch eq₁''
+                                                          all_goals nomatch eq₁''
+                                                        all_goals nomatch eq₁''
+                                                      all_goals nomatch eq₁'
+                                                    all_goals nomatch eq₁
+                                                  | _ + 1 => split at eq₀' <;> nomatch eq₀'
+                                                all_goals nomatch eq₀'
+                                              all_goals nomatch eq₀'
+                                            all_goals nomatch eq₀'
+                                          all_goals nomatch eq₀'
+                                        | _ + 1 => split at eq₀' <;> nomatch eq₀'
+                                      all_goals nomatch eq₀'
+                                    all_goals nomatch eq₀'
+                                  all_goals nomatch eq₀'
+                                all_goals nomatch eq₀'
+                              all_goals nomatch eq₀'
+                            | _ + 1 => split at eq₀' <;> nomatch eq₀'
+                          all_goals nomatch eq₀'
+                        all_goals nomatch eq₀'
+                      all_goals nomatch eq₀'
+                    all_goals nomatch eq₀'
+                  all_goals nomatch eq₀'
+                all_goals nomatch eq₀
+    all_goals nomatch eq
+  all_goals nomatch eq
+
+local instance : Inhabited «Type» where
+  default := .list []
+in
+private
+theorem tc_evidence_eq_inversion (aninA : a ∉ A.freeTypeVars)
+  (A'oplc : (A'.TypeVar_open a).TypeVarLocallyClosed)
+  (Aₛoplc : ∀ i ∈ [:n'], ((Aₛ i).TypeVar_open a).TypeVarLocallyClosed)
+  (Blc : B.TypeVarLocallyClosed)
+  (eq : A.TypeVar_open a n = [[⊗ {A'^^B, </ Aₛ@i^^B // i in [:n'] />}]])
+  : ∃ A'', A' = A''.TypeVar_open a (n + 1) ∧ A = [[⊗ {A''^^B, </ Aₛ@i^^B // i in [:n'] />}]] := by
+  cases A <;> rw [TypeVar_open] at *
+  case prod =>
+    rename «Type» => A
+    let eq' := prod.inj eq
+    cases A <;> rw [TypeVar_open] at *
+    case list =>
+      let eq'' := list.inj eq'
+      rw [List.mapMem_eq_map] at *
+      rename List _ => As
+      match As with
+      | [] => nomatch eq''
+      | A'' :: As' =>
+        rw [List.map_cons] at *
+        let ⟨eq₀, eq₁⟩ := List.cons_eq_cons.mp eq''
+        rw [← Range.map_get!_eq (as := As'), Range.map, List.map_map,
+            List.map_singleton_flatten] at eq₁
+        let length_eq : List.length (List.map ..) = List.length _ :=  by rw [eq₁]
+        rw [List.length_map, List.length_map, Range.length_toList, Range.length_toList,
+            Nat.sub_zero, Nat.sub_zero] at length_eq
+        cases length_eq
+        rw [freeTypeVars, freeTypeVars, List.mapMem_eq_map] at aninA
+        sorry
+        -- let f := List.not_mem_flatten.mp aninA A''.freeTypeVars <| .head _
+        -- let f := Range.eq_of_mem_of_map_eq eq₁
+    all_goals nomatch eq
+  all_goals nomatch eq
+
+end «F⊗⊕ω».Type
 
 open «F⊗⊕ω»
 
+namespace TypeScheme.KindingAndElaboration
+
+theorem weakening : [[Γc; Γ ⊢ σ : κ ⇝ A]] → [[Γc ⊢ Γ, Γ' ⇝ Δ]] → [[Γc; Γ, Γ' ⊢ σ : κ ⇝ A]] := sorry
+
+local instance : Inhabited Monotype where
+  default := .row [] none
+in
+local instance : Inhabited «Type» where
+  default := .list []
+in
+set_option maxHeartbeats 2000000 in
 theorem Monotype_open_preservation
-  (σke : KindingAndElaboration Γc [[(Γ, a : κ₀, Γ')]] (TypeVar_open σ a n) κ₁
+  (σke : KindingAndElaboration Γc [[(Γ, a : κ₀, Γ')]] (TypeVar_open σ a m) κ₁
     (Type.TypeVar_open A a n)) (ΓaΓ'we : [[Γc ⊢ Γ, a : κ₀, Γ' ⇝ Δ]]) (aninΓ' : [[a ∉ dom(Γ')]])
   (aninσ : a ∉ σ.freeTypeVars) (aninA : a ∉ A.freeTypeVars) (τke : [[Γc; Γ ⊢ τ : κ₀ ⇝ B]])
-  : KindingAndElaboration Γc [[(Γ, (Γ' [τ / a]))]] (σ.Monotype_open τ n) κ₁ (A.Type_open B n) := by
-  sorry
+  : KindingAndElaboration Γc [[(Γ, (Γ' [τ / a]))]] (σ.Monotype_open τ m) κ₁ (A.Type_open B n) := by
+  let .qual (.mono τlc) := τke.TypeVarLocallyClosed_of
+  match σ with
+  | .qual γ =>
+    rw [Monotype_open]
+    rw [TypeVar_open] at σke
+    rw [freeTypeVars] at aninσ
+    match h : γ with
+    | .mono τ' =>
+      rw [QualifiedType.Monotype_open]
+      rw [QualifiedType.TypeVar_open] at σke
+      rw [QualifiedType.freeTypeVars] at aninσ
+      match τ' with
+      | .var _ =>
+        rw [Monotype.TypeVar_open] at σke
+        cases A <;> rw [Type.TypeVar_open] at σke
+        case var =>
+          split at σke
+          · case isTrue h =>
+            cases h
+            split at σke
+            · case isTrue h =>
+              cases h
+              rw [Monotype.Monotype_open, if_pos rfl, Type.Type_open, if_pos rfl]
+              let .var ain := σke
+              let .head := ain.append_elim_left aninΓ'
+              exact τke.weakening sorry (Δ := .empty)
+            · case isFalse h =>
+              let .var .. := σke
+              rw [Type.freeTypeVars] at aninA
+              nomatch List.not_mem_singleton.mp aninA
+          · case isFalse h =>
+            split at σke
+            · case isTrue h' =>
+              cases h'
+              let .var .. := σke
+              rw [Monotype.freeTypeVars] at aninσ
+              nomatch List.not_mem_singleton.mp aninσ
+            · case isFalse h' =>
+              rw [Monotype.Monotype_open, if_neg h, Type.Type_open, if_neg h']
+              let .var a'in := σke
+              rw [Type.freeTypeVars] at aninA
+              exact var <| match a'in.append_elim with
+              | .inl ⟨a'inΓa, a'ninΓ'⟩ => match a'inΓa with
+                | .head => nomatch List.not_mem_singleton.mp aninA
+                | .typeExt _ a'inΓ => a'inΓ.append_inl a'ninΓ'.TypeVar_subst_preservation
+              | .inr a'inΓ' => a'inΓ'.TypeVar_subst_preservation.append_inr
+        all_goals split at σke <;> nomatch σke
+      | .app φ τ'' =>
+        rw [Monotype.TypeVar_open] at σke
+        cases A <;> rw [Type.TypeVar_open] at σke
+        case app =>
+          let .app φke τ''ke := σke
+          rw [Monotype.Monotype_open, Type.Type_open]
+          rw [← QualifiedType.TypeVar_open, ← TypeVar_open] at φke τ''ke
+          rw [Monotype.freeTypeVars] at aninσ
+          rw [Type.freeTypeVars] at aninA
+          let φke' := φke.Monotype_open_preservation ΓaΓ'we aninΓ'
+            (aninσ <| List.mem_append_left _ ·) (aninA <| List.mem_append_left _ ·) τke
+          let τ''ke' := τ''ke.Monotype_open_preservation ΓaΓ'we aninΓ'
+            (aninσ <| List.mem_append_right _ ·) (aninA <| List.mem_append_right _ ·) τke
+          rw [Monotype_open, QualifiedType.Monotype_open] at φke' τ''ke'
+          exact app φke' τ''ke'
+        all_goals nomatch σke
+      | .arr τ₀ τ₁ =>
+        rw [Monotype.TypeVar_open] at σke
+        cases A <;> rw [Type.TypeVar_open] at σke
+        case arr =>
+          let .arr τ₀ke τ₁ke := σke
+          rw [Monotype.Monotype_open, Type.Type_open]
+          rw [← QualifiedType.TypeVar_open, ← TypeVar_open] at τ₀ke τ₁ke
+          rw [Monotype.freeTypeVars] at aninσ
+          rw [Type.freeTypeVars] at aninA
+          let τ₀ke' := τ₀ke.Monotype_open_preservation ΓaΓ'we aninΓ'
+            (aninσ <| List.mem_append_left _ ·) (aninA <| List.mem_append_left _ ·) τke
+          let τ₁ke' := τ₁ke.Monotype_open_preservation ΓaΓ'we aninΓ'
+            (aninσ <| List.mem_append_right _ ·) (aninA <| List.mem_append_right _ ·) τke
+          rw [Monotype_open, QualifiedType.Monotype_open] at τ₀ke' τ₁ke'
+          exact arr τ₀ke' τ₁ke'
+        all_goals nomatch σke
+      | .label _ =>
+        rw [Monotype.TypeVar_open] at σke
+        cases A <;> rw [Type.TypeVar_open] at σke
+        case prod =>
+          rw [Monotype.Monotype_open, Type.Type_open]
+          rename «Type» => A
+          cases A <;> rw [Type.TypeVar_open] at σke
+          case list =>
+            rw [Type.Type_open]
+            rw [List.mapMem_eq_map] at σke ⊢
+            rename List _ => As
+            match As with
+            | _ :: _ => nomatch σke
+            | [] =>
+              rw [List.map_nil] at σke ⊢
+              let .label := σke
+              exact label
+          all_goals nomatch σke
+        all_goals nomatch σke
+      | .comm _ =>
+        rw [Monotype.TypeVar_open] at σke
+        cases A <;> rw [Type.TypeVar_open] at σke
+        case prod =>
+          rw [Monotype.Monotype_open, Type.Type_open]
+          rename «Type» => A
+          cases A <;> rw [Type.TypeVar_open] at σke
+          case list =>
+            rw [Type.Type_open]
+            rw [List.mapMem_eq_map] at σke ⊢
+            rename List _ => As
+            match As with
+            | _ :: _ => nomatch σke
+            | [] =>
+              rw [List.map_nil] at σke ⊢
+              let .comm := σke
+              exact comm
+          all_goals nomatch σke
+        all_goals nomatch σke
+      | .row ξτs .. =>
+        rw [Monotype.TypeVar_open, List.mapMem_eq_map] at σke
+        generalize ξτs'eq
+          : (ξτs.map fun (ξ, τ) => (ξ.TypeVar_open a m, τ.TypeVar_open a m)) = ξτs' at σke
+        generalize A'eq : A.TypeVar_open a n = A' at σke
+        let .row ξ'ke uni τ'ke h' (B := B') := σke
+        rw [List.map_singleton_flatten] at ξτs'eq
+        cases A <;> rw [Type.TypeVar_open] at A'eq
+        case list =>
+          rename List _ => A
+          rw [List.mapMem_eq_map, List.map_singleton_flatten] at A'eq
+          let A'eq := Type.list.inj A'eq
+          let ξτslength_eq : List.length (List.map ..) = List.length _ := by rw [ξτs'eq]
+          let Alength_eq : List.length (List.map ..) = List.length _ := by rw [A'eq]
+          rw [List.length_map, List.length_map, Range.length_toList,
+              Nat.sub_zero] at ξτslength_eq Alength_eq
+          let ξ' i := ξτs.get! i |>.fst.Monotype_open τ m
+          let τ' i := ξτs.get! i |>.snd.Monotype_open τ m
+          let A'' i := A.get! i |>.Type_open B n
+          rw [Monotype.Monotype_open, List.mapMem_eq_map, ← Range.map_get!_eq (as := ξτs),
+              ξτslength_eq, Range.map, List.map_map, Type.Type_open, List.mapMem_eq_map,
+              ← Range.map_get!_eq (as := A), Alength_eq, Range.map, List.map_map,
+              Range.map_eq_of_eq_of_mem (by
+                intro i _
+                show _ = (ξ' i, τ' i)
+                simp only [Function.comp]
+              ), ← List.map_singleton_flatten, ← Range.map,
+              Range.map_eq_of_eq_of_mem (by
+                intro i _
+                show _ = A'' i
+                simp only [Function.comp]
+              ), ← List.map_singleton_flatten, ← Range.map]
+          rw [← Range.map_get!_eq (as := ξτs), ξτslength_eq, Range.map, List.map_map] at ξτs'eq
+          rw [Monotype.freeTypeVars, List.mapMem_eq_map] at aninσ
+          let aninξ i ilt : a ∉ (ξτs.get! i).fst.freeTypeVars := by
+            apply (List.not_mem_append' (xs := (ξτs.get! i).snd.freeTypeVars)).mp _ |>.right
+            apply List.not_mem_flatten.mp aninσ
+            apply List.mem_map.mpr
+            exact ⟨_, List.get!_mem ilt, rfl⟩
+          let aninτ i ilt : a ∉ (ξτs.get! i).snd.freeTypeVars := by
+            apply (List.not_mem_append' (ys := (ξτs.get! i).fst.freeTypeVars)).mp _ |>.left
+            apply List.not_mem_flatten.mp aninσ
+            apply List.mem_map.mpr
+            exact ⟨_, List.get!_mem ilt, rfl⟩
+          apply row (B := fun i => ((B' i).TypeVar_close a m).Type_open B m) _ _ _ h'
+          · intro i mem
+            dsimp only [ξ']
+            let ξike := ξ'ke i mem
+            simp only at ξike
+            have := Range.eq_of_mem_of_map_eq ξτs'eq i mem
+            simp only [Function.comp] at this
+            rw [← Prod.mk.inj this |>.left, ← QualifiedType.TypeVar_open, ← TypeVar_open] at ξike
+            let Bki := ξike.soundness ΓaΓ'we .label |>.TypeVarLocallyClosed_of.weaken (n := m)
+            rw [Nat.zero_add] at Bki
+            rw [← Bki.TypeVar_open_TypeVar_close_id (a := a)] at ξike
+            let ilt : i < ξτs.length := by rw [ξτslength_eq]; exact mem.right
+            have := ξike.Monotype_open_preservation ΓaΓ'we aninΓ' (aninξ i ilt)
+              Type.not_mem_freeTypeVars_TypeVar_close τke
+            rw [Monotype_open, QualifiedType.Monotype_open] at this
+            exact this
+          · rw [List.map_singleton_flatten, funext (f := ξ') (by
+              intro i
+              show _ = ((fun x => x.Monotype_open τ m) ∘ (fun i => ξτs.get! i |>.fst)) i
+              simp only [ξ', Function.comp]
+            ), ← List.map_map]
+            apply Monotype.label.Uniqueness.Monotype_open_preservation (a := a)
+            rw [Range.map, List.map_singleton_flatten, Range.map_eq_of_eq_of_mem (by
+              intro i mem
+              have := Range.eq_of_mem_of_map_eq ξτs'eq i mem
+              simp only [Function.comp] at this
+              rw [← Prod.mk.inj this |>.left]
+            )] at uni
+            rw [List.map_map, ← Range.map, Range.map, Range.map_eq_of_eq_of_mem (by
+              intro i mem
+              show _ = (ξτs.get! i).fst.TypeVar_open a m
+              simp only [Function.comp]
+            )]
+            exact uni
+          · intro i mem
+            dsimp only [τ', A'']
+            let τike := τ'ke i mem
+            simp only at τike
+            have := Range.eq_of_mem_of_map_eq ξτs'eq i mem
+            simp only [Function.comp] at this
+            rw [← Prod.mk.inj this |>.right, ← QualifiedType.TypeVar_open, ← TypeVar_open] at τike
+            rw [← Range.map_get!_eq (as := A), Range.map, List.map_map, Alength_eq] at A'eq
+            have := Range.eq_of_mem_of_map_eq A'eq i mem
+            simp only [Function.comp] at this
+            rw [← this] at τike
+            rw [Type.freeTypeVars, List.mapMem_eq_map] at aninA
+            have iltAlength : i < A.length := by
+              rw [Alength_eq]
+              exact mem.right
+            let aninAi := List.not_mem_flatten.mp aninA (A.get! i).freeTypeVars
+              (List.mem_map.mpr ⟨_, List.get!_mem iltAlength, rfl⟩)
+            let ilt : i < ξτs.length := by rw [ξτslength_eq]; exact mem.right
+            have := τike.Monotype_open_preservation ΓaΓ'we aninΓ' (aninτ i ilt) aninAi τke
+            rw [Monotype_open, QualifiedType.Monotype_open] at this
+            exact this
+        all_goals nomatch A'eq
+      | .floor _ =>
+        rw [Monotype.TypeVar_open] at σke
+        cases A <;> rw [Type.TypeVar_open] at σke
+        case prod =>
+          rw [Monotype.Monotype_open, Type.Type_open]
+          rename «Type» => A
+          cases A <;> rw [Type.TypeVar_open] at σke
+          case list =>
+            rw [Type.Type_open]
+            rw [List.mapMem_eq_map] at σke ⊢
+            rename List _ => As
+            match As with
+            | _ :: _ => nomatch σke
+            | [] =>
+              rw [List.map_nil] at σke ⊢
+              let .floor ξke := σke
+              rw [← QualifiedType.TypeVar_open, ← TypeVar_open] at ξke
+              let Alc := ξke.soundness ΓaΓ'we .label |>.TypeVarLocallyClosed_of.weaken (n := n)
+              rw [Nat.zero_add] at Alc
+              rw [← Alc.TypeVar_open_TypeVar_close_id (a := a)] at ξke
+              rw [Monotype.freeTypeVars] at aninσ
+              exact floor <| ξke.Monotype_open_preservation ΓaΓ'we aninΓ' aninσ
+                Type.not_mem_freeTypeVars_TypeVar_close τke
+          all_goals nomatch σke
+        all_goals nomatch σke
+      | .prod .. =>
+        rw [Monotype.TypeVar_open] at σke
+        cases A <;> rw [Type.TypeVar_open] at σke
+        case prod =>
+          let .prod μke ρke := σke
+          rw [Monotype.Monotype_open, Type.Type_open]
+          rw [← QualifiedType.TypeVar_open, ← TypeVar_open] at μke ρke
+          rw [Monotype.freeTypeVars] at aninσ
+          rw [Type.freeTypeVars] at aninA
+          let Blc := μke.soundness ΓaΓ'we .comm |>.TypeVarLocallyClosed_of.weaken (n := n)
+          rw [Nat.zero_add] at Blc
+          rw [← Blc.TypeVar_open_TypeVar_close_id (a := a)] at μke
+          let μke' := μke.Monotype_open_preservation ΓaΓ'we aninΓ'
+            (aninσ <| List.mem_append_left _ ·) Type.not_mem_freeTypeVars_TypeVar_close τke
+          let ρke' := ρke.Monotype_open_preservation ΓaΓ'we aninΓ'
+            (aninσ <| List.mem_append_right _ ·) aninA τke
+          rw [Monotype_open, QualifiedType.Monotype_open] at μke' ρke'
+          exact prod μke' ρke'
+        all_goals nomatch σke
+      | .sum .. =>
+        rw [Monotype.TypeVar_open] at σke
+        cases A <;> rw [Type.TypeVar_open] at σke
+        case sum =>
+          let .sum μke ρke := σke
+          rw [Monotype.Monotype_open, Type.Type_open]
+          rw [← QualifiedType.TypeVar_open, ← TypeVar_open] at μke ρke
+          rw [Monotype.freeTypeVars] at aninσ
+          rw [Type.freeTypeVars] at aninA
+          let Blc := μke.soundness ΓaΓ'we .comm |>.TypeVarLocallyClosed_of.weaken (n := n)
+          rw [Nat.zero_add] at Blc
+          rw [← Blc.TypeVar_open_TypeVar_close_id (a := a)] at μke
+          let μke' := μke.Monotype_open_preservation ΓaΓ'we aninΓ'
+            (aninσ <| List.mem_append_left _ ·) Type.not_mem_freeTypeVars_TypeVar_close τke
+          let ρke' := ρke.Monotype_open_preservation ΓaΓ'we aninΓ'
+            (aninσ <| List.mem_append_right _ ·) aninA τke
+          rw [Monotype_open, QualifiedType.Monotype_open] at μke' ρke'
+          exact sum μke' ρke'
+        all_goals nomatch σke
+      | .lift .. =>
+        rename TypeLambda => «λτ»
+        let .mk _ τ'' := «λτ»
+        rw [Monotype.TypeVar_open, TypeLambda.TypeVar_open] at σke
+        cases A <;> rw [Type.TypeVar_open] at σke
+        case listApp =>
+          rename_i A _
+          cases A <;> rw [Type.TypeVar_open] at σke
+          case lam =>
+            rename «Type» => A
+            let .lift I τ''ke κ₀'e ρke := σke
+            rw [Monotype.Monotype_open, TypeLambda.Monotype_open, Type.Type_open, Type.Type_open]
+            rw [← QualifiedType.TypeVar_open, ← TypeVar_open] at ρke
+            rw [Monotype.freeTypeVars, TypeLambda.freeTypeVars] at aninσ
+            rw [Type.freeTypeVars, Type.freeTypeVars] at aninA
+            let ρke' := ρke.Monotype_open_preservation ΓaΓ'we aninΓ'
+              (aninσ <| List.mem_append_right _ ·) (aninA <| List.mem_append_right _ ·) τke
+            rw [Monotype_open, QualifiedType.Monotype_open] at ρke'
+            apply lift ([[(Γ, a : κ₀, Γ')]].typeVarDom ++ I) _ κ₀'e ρke'
+            intro a' a'nin
+            let ⟨a'ninΓaΓ'', a'ninI⟩ := List.not_mem_append'.mp a'nin
+            have a'ninΓa : [[a' ∉ dom(Γ, a : κ₀)]] := by
+              rw [TypeEnvironment.typeVarDom_append] at a'ninΓaΓ''
+              exact List.not_mem_append'.mp a'ninΓaΓ'' |>.right
+            let ne := List.ne_of_not_mem_cons a'ninΓa
+            symm at ne
+            let ⟨_, .typeExt Γwe ..⟩ := ΓaΓ'we.append_left_elim
+            let ⟨_, κ₀e⟩ := κ₀.Elaboration_total
+            let Blc := τke.soundness Γwe κ₀e |>.TypeVarLocallyClosed_of
+            rw [Blc.Type_open_TypeVar_open_comm <| Nat.succ_ne_zero _]
+            have := τ''ke a' a'ninI
+            rw [τ''.TypeVar_open_comm <| Nat.succ_ne_zero _,
+                ← QualifiedType.TypeVar_open, ← TypeVar_open,
+                A.TypeVar_open_comm <| Nat.succ_ne_zero _, ← TypeEnvironment.append] at this
+            have := this.Monotype_open_preservation (ΓaΓ'we.typeExt a'ninΓaΓ'' κ₀'e)
+               (List.not_mem_cons.mpr ⟨ne, aninΓ'⟩)
+               (Monotype.not_mem_freeTypeVars_TypeVar_open_intro
+                 (aninσ <| List.mem_append_left _ ·) ne)
+               (Type.not_mem_freeTypeVars_TypeVar_open_intro
+                 (aninA <| List.mem_append_left _ ·) ne) τke
+            rw [← TypeEnvironment.append, ← TypeEnvironment.TypeVar_subst,
+                ← τ''.TypeVar_open_Monotype_open_comm τlc <| Nat.zero_ne_add_one _,
+                ← QualifiedType.Monotype_open, ← Monotype_open]
+            exact this
+          all_goals nomatch σke
+        all_goals nomatch σke
+      | .contain .. =>
+        rw [Monotype.TypeVar_open] at σke
+        generalize A'eq : A.TypeVar_open a n = A' at σke
+        let .contain μke ρ₀ke ρ₁ke κe := σke
+        let ⟨A₀, A₁, eq₀, eq₁, eq₂⟩ := Type.contain_evidence_eq_inversion aninA A'eq
+        cases eq₀
+        cases eq₁
+        cases eq₂
+        clear A'eq
+        rw [Monotype.Monotype_open, Type.Type_open, Type.Type_open, List.mapMem_eq_map,
+            List.map_cons, List.map_singleton]
+        repeat rw [Type.Type_open]
+        rw [if_neg (nomatch ·)]
+        rw [← QualifiedType.TypeVar_open, ← TypeVar_open] at μke ρ₀ke ρ₁ke
+        rw [Monotype.freeTypeVars] at aninσ
+        let ⟨aninρ₀μ, aninρ₁⟩ := List.not_mem_append'.mp aninσ
+        let ⟨aninρ₀, aninμ⟩ := List.not_mem_append'.mp aninρ₀μ
+        simp [Type.freeTypeVars] at aninA
+        let ⟨_, aninA₀, aninA₁⟩ := aninA
+        let Blc := μke.soundness ΓaΓ'we .comm |>.TypeVarLocallyClosed_of.weaken (n := n)
+        rw [Nat.zero_add] at Blc
+        rw [← Blc.TypeVar_open_TypeVar_close_id (a := a)] at μke
+        let μke' := μke.Monotype_open_preservation ΓaΓ'we aninΓ' aninμ
+          Type.not_mem_freeTypeVars_TypeVar_close τke
+        let ρ₀ke' := ρ₀ke.Monotype_open_preservation ΓaΓ'we aninΓ' aninρ₀ aninA₀ τke
+        let ρ₁ke' := ρ₁ke.Monotype_open_preservation ΓaΓ'we aninΓ' aninρ₁ aninA₁ τke
+        rw [Monotype_open, QualifiedType.Monotype_open] at ρ₀ke' ρ₁ke'
+        exact contain μke' ρ₀ke' ρ₁ke' κe
+      | .concat .. =>
+        rw [Monotype.TypeVar_open] at σke
+        generalize A'eq : A.TypeVar_open a n = A' at σke
+        let .concat μke ρ₀ke ρ₁ke ρ₂ke κe _ _ := σke
+        let foo := Type.concat_evidence_eq_inversion aninA A'eq
+        sorry
+        -- cases eq₀
+        -- cases eq₁
+        -- cases eq₂
+        -- clear A'eq
+        -- rw [Monotype.Monotype_open, Type.Type_open, Type.Type_open, List.mapMem_eq_map,
+        --     List.map_cons, List.map_singleton]
+        -- repeat rw [Type.Type_open]
+        -- rw [if_neg (nomatch ·)]
+        -- rw [← QualifiedType.TypeVar_open, ← TypeVar_open] at μke ρ₀ke ρ₁ke
+        -- rw [Monotype.freeTypeVars] at aninσ
+        -- let ⟨aninρ₀μ, aninρ₁⟩ := List.not_mem_append'.mp aninσ
+        -- let ⟨aninρ₀, aninμ⟩ := List.not_mem_append'.mp aninρ₀μ
+        -- simp [Type.freeTypeVars] at aninA
+        -- let ⟨_, aninA₀, aninA₁⟩ := aninA
+        -- let Blc := μke.soundness ΓaΓ'we .comm |>.TypeVarLocallyClosed_of.weaken (n := n)
+        -- rw [Nat.zero_add] at Blc
+        -- rw [← Blc.TypeVar_open_TypeVar_close_id (a := a)] at μke
+        -- let μke' := μke.Monotype_open_preservation ΓaΓ'we aninΓ' aninμ
+        --   Type.not_mem_freeTypeVars_TypeVar_close τke
+        -- let ρ₀ke' := ρ₀ke.Monotype_open_preservation ΓaΓ'we aninΓ' aninρ₀ aninA₀ τke
+        -- let ρ₁ke' := ρ₁ke.Monotype_open_preservation ΓaΓ'we aninΓ' aninρ₁ aninA₁ τke
+        -- rw [Monotype_open, QualifiedType.Monotype_open] at ρ₀ke' ρ₁ke'
+        -- exact contain μke' ρ₀ke' ρ₁ke' κe
+      | .typeClass .. =>
+        rw [Monotype.TypeVar_open] at σke
+        generalize A'eq : A.TypeVar_open a n = A' at σke
+        let .tc Γcw inΓc τ'ke (κ := κ) := σke
+        let ⟨_, κe⟩ := κ.Elaboration_total
+        let ⟨Aki, Aₛki⟩ := Γcw.KindingAndElaboration_of_ClassEnvironment_in inΓc κe a
+        let B'lc := τ'ke.soundness ΓaΓ'we κe |>.TypeVarLocallyClosed_of
+        let ⟨_, eq⟩ := Type.tc_evidence_eq_inversion aninA Aki.TypeVarLocallyClosed_of
+          (Aₛki · · |>.TypeVarLocallyClosed_of) B'lc A'eq
+        sorry
+      | .all .. =>
+        rename TypeLambda => «λτ»
+        let .mk _ ψ := «λτ»
+        rw [Monotype.TypeVar_open, TypeLambda.TypeVar_open] at σke
+        cases A <;> rw [Type.TypeVar_open] at σke
+        case prod =>
+          rename «Type» => A
+          cases A <;> rw [Type.TypeVar_open] at σke
+          case listApp =>
+            rename_i A _
+            cases A <;> rw [Type.TypeVar_open] at σke
+            case lam =>
+              rename «Type» => A
+              let .all I ψke κe ρke := σke
+              rw [Monotype.Monotype_open, TypeLambda.Monotype_open, Type.Type_open, Type.Type_open,
+                  Type.Type_open]
+              rw [← QualifiedType.TypeVar_open, ← TypeVar_open] at ρke
+              rw [Monotype.freeTypeVars, TypeLambda.freeTypeVars] at aninσ
+              rw [Type.freeTypeVars, Type.freeTypeVars, Type.freeTypeVars] at aninA
+              let ρke' := ρke.Monotype_open_preservation ΓaΓ'we aninΓ'
+                (aninσ <| List.mem_append_right _ ·) (aninA <| List.mem_append_right _ ·) τke
+              rw [Monotype_open, QualifiedType.Monotype_open] at ρke'
+              apply all ([[(Γ, a : κ₀, Γ')]].typeVarDom ++ I) _ κe ρke'
+              intro a' a'nin
+              let ⟨a'ninΓaΓ'', a'ninI⟩ := List.not_mem_append'.mp a'nin
+              have a'ninΓa : [[a' ∉ dom(Γ, a : κ₀)]] := by
+                rw [TypeEnvironment.typeVarDom_append] at a'ninΓaΓ''
+                exact List.not_mem_append'.mp a'ninΓaΓ'' |>.right
+              let ne := List.ne_of_not_mem_cons a'ninΓa
+              symm at ne
+              let ⟨_, .typeExt Γwe ..⟩ := ΓaΓ'we.append_left_elim
+              let ⟨_, κ₀e⟩ := κ₀.Elaboration_total
+              let Blc := τke.soundness Γwe κ₀e |>.TypeVarLocallyClosed_of
+              rw [Blc.Type_open_TypeVar_open_comm <| Nat.succ_ne_zero _]
+              have := ψke a' a'ninI
+              rw [ψ.TypeVar_open_comm <| Nat.succ_ne_zero _,
+                  ← QualifiedType.TypeVar_open, ← TypeVar_open,
+                  A.TypeVar_open_comm <| Nat.succ_ne_zero _, ← TypeEnvironment.append] at this
+              have := this.Monotype_open_preservation (ΓaΓ'we.typeExt a'ninΓaΓ'' κe)
+                (List.not_mem_cons.mpr ⟨ne, aninΓ'⟩)
+                (Monotype.not_mem_freeTypeVars_TypeVar_open_intro
+                  (aninσ <| List.mem_append_left _ ·) ne)
+                (Type.not_mem_freeTypeVars_TypeVar_open_intro
+                  (aninA <| List.mem_append_left _ ·) ne) τke
+              rw [← TypeEnvironment.append, ← TypeEnvironment.TypeVar_subst,
+                  ← ψ.TypeVar_open_Monotype_open_comm τlc <| Nat.zero_ne_add_one _,
+                  ← QualifiedType.Monotype_open, ← Monotype_open]
+              exact this
+            all_goals nomatch σke
+          all_goals nomatch σke
+        all_goals nomatch σke
+      | .ind .. => sorry
+      | .split (.mk κ τ'') ρ₀ ρ₁ ρ₂ =>
+        rw [Monotype.TypeVar_open, TypeLambda.TypeVar_open] at σke
+        let .split concatke := σke
+        rw [Monotype.Monotype_open, TypeLambda.Monotype_open]
+        let concatke' : KindingAndElaboration _ _ (TypeVar_open
+            (.qual (.mono (.concat (.lift (.mk _ τ'') ρ₀) (.comm .comm) ρ₁ ρ₂))) a m) .. := by
+          rw [TypeVar_open, QualifiedType.TypeVar_open, Monotype.TypeVar_open,
+              Monotype.TypeVar_open, Monotype.TypeVar_open, TypeLambda.TypeVar_open]
+          exact concatke
+        rw [Monotype.freeTypeVars] at aninσ
+        let concatke'' := concatke'.Monotype_open_preservation ΓaΓ'we aninΓ' (by
+            rw [freeTypeVars, QualifiedType.freeTypeVars, Monotype.freeTypeVars,
+                Monotype.freeTypeVars, Monotype.freeTypeVars, List.append_nil]
+            exact aninσ
+          ) aninA τke
+        rw [Monotype_open, QualifiedType.Monotype_open, Monotype.Monotype_open,
+            Monotype.Monotype_open, Monotype.Monotype_open, TypeLambda.Monotype_open] at concatke''
+        exact split concatke''
+    | .qual ψ γ' =>
+      rw [QualifiedType.TypeVar_open] at σke
+      cases A <;> rw [Type.TypeVar_open] at σke
+      case arr =>
+        let .qual ψke γ'ke κ₁e := σke
+        rw [QualifiedType.Monotype_open, Type.Type_open]
+        rw [← QualifiedType.TypeVar_open] at ψke
+        rw [← TypeVar_open] at ψke γ'ke
+        rw [Type.freeTypeVars] at aninA
+        let ψke' := ψke.Monotype_open_preservation ΓaΓ'we aninΓ' (aninσ <| List.mem_append_left _ ·)
+          (aninA <| List.mem_append_left _ ·) τke
+        let γ'ke' := γ'ke.Monotype_open_preservation ΓaΓ'we aninΓ'
+          (aninσ <| List.mem_append_right _ ·) (aninA <| List.mem_append_right _ ·) τke
+        rw [Monotype_open] at ψke' γ'ke'
+        rw [QualifiedType.Monotype_open] at ψke'
+        exact qual ψke' γ'ke' κ₁e
+      all_goals nomatch σke
+  | .quant κ σ' =>
+    rw [TypeVar_open] at σke
+    cases A <;> rw [Type.TypeVar_open] at σke
+    case var => split at σke <;> nomatch σke
+    case «forall» K A =>
+      let .scheme I σ'ke κe := σke
+      rw [Monotype_open, Type.Type_open]
+      apply scheme ([[(Γ, a : κ₀, Γ')]].typeVarDom ++ I) _ κe
+      intro a' a'nin
+      let ⟨a'ninΓaΓ'', a'ninI⟩ := List.not_mem_append'.mp a'nin
+      have a'ninΓa : [[a' ∉ dom(Γ, a : κ₀)]] := by
+        rw [TypeEnvironment.typeVarDom_append] at a'ninΓaΓ''
+        exact List.not_mem_append'.mp a'ninΓaΓ'' |>.right
+      let ne := List.ne_of_not_mem_cons a'ninΓa
+      symm at ne
+      let ⟨_, .typeExt Γwe ..⟩ := ΓaΓ'we.append_left_elim
+      let ⟨_, κ₀e⟩ := κ₀.Elaboration_total
+      let Blc := τke.soundness Γwe κ₀e |>.TypeVarLocallyClosed_of
+      rw [Blc.Type_open_TypeVar_open_comm <| Nat.succ_ne_zero _]
+      have := σ'ke a' a'ninI
+      rw [σ'.TypeVar_open_comm <| Nat.succ_ne_zero _,
+          A.TypeVar_open_comm <| Nat.succ_ne_zero _, ← TypeEnvironment.append] at this
+      rw [freeTypeVars] at aninσ
+      rw [Type.freeTypeVars] at aninA
+      have := this.Monotype_open_preservation (ΓaΓ'we.typeExt a'ninΓaΓ'' κe)
+        (List.not_mem_cons.mpr ⟨ne, aninΓ'⟩) (not_mem_freeTypeVars_TypeVar_open_intro aninσ ne)
+        (Type.not_mem_freeTypeVars_TypeVar_open_intro aninA ne) τke
+      rw [← TypeEnvironment.append, ← TypeEnvironment.TypeVar_subst,
+          ← σ'.TypeVar_open_Monotype_open_comm τlc <| Nat.zero_ne_add_one _]
+      exact this
+    all_goals nomatch σke
+termination_by σ.sizeOf'
+decreasing_by
+  all_goals simp_arith; try simp_arith [h]
+  · rw [← List.get!_eq_getElem!]
+    apply Nat.le_add_right_of_le
+    apply Nat.le_of_add_right_le (k := (ξτs.get! i).snd.sizeOf')
+    apply List.le_sum_of_mem'
+    apply List.mem_map.mpr
+    exact ⟨_, List.get!_mem ilt, rfl⟩
+  · rw [← List.get!_eq_getElem!]
+    apply Nat.le_add_right_of_le
+    apply Nat.le_of_add_right_le (k := (ξτs.get! i).fst.sizeOf')
+    rw [Nat.add_comm]
+    apply List.le_sum_of_mem'
+    apply List.mem_map.mpr
+    exact ⟨_, List.get!_mem ilt, rfl⟩
+  · exact Nat.succ_le_of_lt <| QualifiedType.sizeOf'_pos _
 
-end TabularTypeInterpreter.TypeScheme.KindingAndElaboration
+end TypeScheme.KindingAndElaboration
+
+end TabularTypeInterpreter
